Expand hocap-logatom equivalence proof + discussion

theories/logatom/elimination_stack/hocap_spec.v
@@ -1,3 +1,34 @@
+(** This file explores the relation between "logically atomic"-style specs and
+HoCAP-style specs.  The key difference between these specs is as follows:
+- Logically atomic specs require the client to prove a mask-changing view shift
+  which, at the linearization point, gets used to access the atomic
+  precondition. The client can open invariants to prove this view shift. The
+  library then works with this precondition, transforms it to the postcondition
+  (which usually involves changing the abstract state), and gives that back to
+  the client for a "closing" mask-changing view shift, where the client can
+  close the invariants again.
+- HoCAP-style specs require the client to prove a non-mask-changing view shift
+  which may assume as an assumption the "old" abstract state of the library, and
+  has to produce the "new" abstract state. Unlike with logically atomic specs,
+  it is up to the *client* to change the abstract state to match the current
+  operation. This pattern also does not really have a notion of "atomic
+  precondition"; the relation between a sequential specification and its atomic
+  counterpart is much more complex with HoCAP-style specs than it is with
+  logically atomic specs.
+
+One consequence of this difference is that there are some specs where the HoCAP
+style simply does not work: one cannot use the HoCAP style to prove a spec about
+the abstraction of *another library*.  See
+<https://people.mpi-sws.org/~jung/iris/logatom-talk-2019.pdf#page=89> and
+[heap_lang.lib.increment] in the Iris repository for an example of this.
+
+For libraries that only state atomic transitions for their own abstraction, the
+two styles are equivalent, as this file shows: we give two different HoCAP-style
+specs (the "authoritative" variant, which is closer to the original HoCAP paper,
+and the "predicate" variant which is somewhat simpler), and we show them both
+equivalent to the logically atomic spec. *)
+
+
 From stdpp Require Import namespaces.
 From iris.algebra Require Import excl auth list.
 From iris.base_logic.lib Require Import invariants.
@@ -18,8 +49,11 @@ Module logatom := elimination_stack.spec.
 - We also slightly weaken the spec by adding [make_laterable], which is needed
   because logical atomicity can only capture laterable resources, which is
   needed when implementing e.g. the elimination stack on top of an abstract
-  logically atomic heap. *)
-Record hocap_stack {Σ} `{!heapG Σ} := AtomicStack {
+  logically atomic heap.
+
+This spec follows the "authoritative" variant of HoCAP specs. *)
+Module hocap_auth.
+Record stack {Σ} `{!heapG Σ} := AtomicStack {
   (* -- operations -- *)
   new_stack : val;
   push : val;
@@ -60,15 +94,275 @@ Record hocap_stack {Σ} `{!heapG Σ} := AtomicStack {
                 | v :: l' => stack_content_auth γs l' ∗ Φ (SOMEV v) end) -∗
     WP pop s {{ Φ }};
 }.
-Arguments hocap_stack _ {_}.
+Arguments stack _ {_}.
 
 Existing Instances
   is_stack_persistent stack_content_frag_timeless stack_content_auth_timeless
   name_eqdec name_countable.
 
+End hocap_auth.
+
+(** A general HoCAP-style interface for a stack. This spec follows
+the "predicate" variant of HoCAP specs. *)
+Module hocap_pred.
+Record stack {Σ} `{!heapG Σ} := AtomicStack {
+  (* -- operations -- *)
+  new_stack : val;
+  push : val;
+  pop : val;
+  (* -- predicates -- *)
+  is_stack (N : namespace) (v : val) (P : list val → iProp Σ) : iProp Σ;
+  (* -- predicate properties -- *)
+  is_stack_persistent N P v : Persistent (is_stack N P v);
+  is_stack_ne N v n : Proper (pointwise_relation _ (dist n) ==> dist n) (is_stack N v);
+  (* -- operation specs -- *)
+  new_stack_spec N P :
+    {{{ ▷ P [] }}} new_stack #() {{{ s, RET s; is_stack N s P }}};
+  push_spec N s P (v : val) (Φ : val → iProp Σ) :
+    is_stack N s P -∗
+    make_laterable (∀ l, ▷ P l ={⊤∖↑N}=∗ ▷ P (v::l) ∗ Φ #()) -∗
+    WP push s v {{ Φ }};
+  pop_spec N s P (Φ : val → iProp Σ) :
+    is_stack N s P -∗
+    make_laterable (∀ l, ▷ P l ={⊤∖↑N}=∗
+          match l with [] => ▷ P [] ∗ Φ NONEV
+                | v :: l' => ▷ P l' ∗ Φ (SOMEV v) end) -∗
+    WP pop s {{ Φ }};
+}.
+Arguments stack _ {_}.
+
+Existing Instances is_stack_persistent.
+
+End hocap_pred.
+
+(** Now we show the following three implications:
+- hocap_auth implies logatom.
+- logcatom implies hocap_pred.
+- hocap_pred implies hocap_auth.
+*)
+
+
+(** From a HoCAP-"auth" stack we can directly implement the logically atomic
+interface.
+
+Roughly:
+logatom.is_stack := hocap_auth.is_stack
+logatom.stack_content := hocap_auth.stack_content_frag
+*)
+Section hocap_auth_logatom.
+  Context `{!heapG Σ} (stack: hocap_auth.stack Σ).
+
+  Lemma logatom_push N γs s (v : val) :
+    stack.(hocap_auth.is_stack) N γs s -∗
+    <<< ∀ l : list val, stack.(hocap_auth.stack_content_frag) γs l >>>
+      stack.(hocap_auth.push) s v @ ⊤∖↑N
+    <<< stack.(hocap_auth.stack_content_frag) γs (v::l), RET #() >>>.
+  Proof.
+    iIntros "Hstack". iIntros (Φ) "HΦ".
+    iApply (hocap_auth.push_spec with "Hstack").
+    iApply (make_laterable_intro with "[] HΦ"). iIntros "!# >HΦ" (l) "Hauth".
+    iMod "HΦ" as (l') "[Hfrag [_ Hclose]]".
+    iDestruct (hocap_auth.stack_content_agree with "Hfrag Hauth") as %->.
+    iMod (hocap_auth.stack_content_update with "Hfrag Hauth") as "[Hfrag $]".
+    iMod ("Hclose" with "Hfrag") as "HΦ". done.
+  Qed.
+
+  Lemma logatom_pop N γs (s : val) :
+    stack.(hocap_auth.is_stack) N γs s -∗
+    <<< ∀ l : list val, stack.(hocap_auth.stack_content_frag) γs l >>>
+      stack.(hocap_auth.pop) s @ ⊤∖↑N
+    <<< stack.(hocap_auth.stack_content_frag) γs (tail l),
+        RET match l with [] => NONEV | v :: _ => SOMEV v end >>>.
+  Proof.
+    iIntros "Hstack". iIntros (Φ) "HΦ".
+    iApply (hocap_auth.pop_spec with "Hstack").
+    iApply (make_laterable_intro with "[] HΦ"). iIntros "!# >HΦ" (l) "Hauth".
+    iMod "HΦ" as (l') "[Hfrag [_ Hclose]]".
+    iDestruct (hocap_auth.stack_content_agree with "Hfrag Hauth") as %->.
+    destruct l;
+    iMod (hocap_auth.stack_content_update with "Hfrag Hauth") as "[Hfrag $]";
+    iMod ("Hclose" with "Hfrag") as "HΦ"; done.
+  Qed.
+
+  Definition hocap_auth_logatom : logatom.atomic_stack Σ :=
+    {| logatom.new_stack_spec := stack.(hocap_auth.new_stack_spec);
+       logatom.push_spec := logatom_push;
+       logatom.pop_spec := logatom_pop;
+       logatom.stack_content_exclusive := stack.(hocap_auth.stack_content_frag_exclusive) |}.
+
+End hocap_auth_logatom.
+
+(** From a logically atomic stack, we can implement a HoCAP-"pred" stack by
+ adding an invariant.
+
+Roughly:
+hocap_pred.is_stack P := logatom.is_stack * inv (∃ l, logatom.stack_content l * P l)
+*)
+Section logatom_hocap_pred.
+  Context `{!heapG Σ} (stack: logatom.atomic_stack Σ).
+  Implicit Type P : list val → iProp Σ.
+
+  Definition hocap_pred_is_stack N v P : iProp Σ :=
+    (∃ γs, stack.(logatom.is_stack) (N .@ "stack") γs v ∗
+     inv (N .@ "wrapper") (∃ l, stack.(logatom.stack_content) γs l ∗ P l))%I.
+
+  Instance hocap_pred_is_stack_ne N v n :
+    Proper (pointwise_relation _ (dist n) ==> dist n) (hocap_pred_is_stack N v).
+  Proof. solve_proper. Qed.
+
+  Lemma hocap_pred_new_stack N P :
+    {{{ ▷ P [] }}}
+      stack.(logatom.new_stack) #()
+    {{{ s, RET s; hocap_pred_is_stack N s P }}}.
+  Proof.
+    iIntros (Φ) "HP HΦ". iApply wp_fupd. iApply logatom.new_stack_spec; first done.
+    iIntros "!>" (γs s) "[Hstack Hcont]".
+    iApply "HΦ". rewrite /hocap_pred_is_stack. iExists γs. iFrame.
+    iApply inv_alloc. eauto with iFrame.
+  Qed.
+
+  Lemma hocap_pred_push N s P (v : val) (Φ : val → iProp Σ) :
+    hocap_pred_is_stack N s P -∗
+    make_laterable (∀ l, ▷ P l ={⊤∖↑N}=∗ ▷ P (v::l) ∗ Φ #()) -∗
+    WP stack.(logatom.push) s v {{ Φ }}.
+  Proof.
+    iIntros "#Hstack Hupd". iDestruct "Hstack" as (γs) "[Hstack Hinv]".
+    awp_apply (logatom.push_spec with "Hstack").
+    iInv "Hinv" as (l) "[>Hcont HP]".
+    iAaccIntro with "Hcont"; first by eauto 10 with iFrame.
+    iIntros "Hcont".
+    iMod fupd_intro_mask' as "Hclose";
+      last iMod (make_laterable_elim with "Hupd HP") as "[HP HΦ]"; first solve_ndisj.
+    iMod "Hclose" as "_". iIntros "!>".
+    eauto with iFrame.
+  Qed.
+
+  Lemma hocap_pred_pop N s P (Φ : val → iProp Σ) :
+    hocap_pred_is_stack N s P -∗
+    make_laterable (∀ l, ▷ P l ={⊤∖↑N}=∗
+          match l with [] => ▷ P [] ∗ Φ NONEV
+                | v :: l' => ▷ P l' ∗ Φ (SOMEV v) end) -∗
+    WP stack.(logatom.pop) s {{ Φ }}.
+  Proof.
+    iIntros "#Hstack Hupd". iDestruct "Hstack" as (γs) "[Hstack Hinv]".
+    awp_apply (logatom.pop_spec with "Hstack").
+    iInv "Hinv" as (l) "[>Hcont HP]".
+    iAaccIntro with "Hcont"; first by eauto 10 with iFrame.
+    iIntros "Hcont". destruct l.
+    - iMod fupd_intro_mask' as "Hclose";
+        last iMod (make_laterable_elim with "Hupd HP") as "[HP HΦ]"; first solve_ndisj.
+       iMod "Hclose" as "_". iIntros "!>"; eauto with iFrame.
+    - iMod fupd_intro_mask' as "Hclose";
+        last iMod (make_laterable_elim with "Hupd HP") as "[HP HΦ]"; first solve_ndisj.
+       iMod "Hclose" as "_". iIntros "!>"; eauto with iFrame.
+  Qed.
+
+  Program Definition logatom_hocap_pred : hocap_pred.stack Σ :=
+    {| hocap_pred.new_stack_spec := hocap_pred_new_stack;
+       hocap_pred.push_spec := hocap_pred_push;
+       hocap_pred.pop_spec := hocap_pred_pop |}.
+
+End logatom_hocap_pred.
+
+(** From a hocap_pred stack, we can implement a hocap_auth stack by adding an
+auth.
+
+Roughly:
+hocap_auth.is_stack := hocap_pred.is_stack (λ l, auth l)
+hocap_auth.stack_content_auth := auth
+hocap_auth.stack_content_frag := frag
+*)
+
+(** The CMRA & functor we need. *)
+Class hocapG Σ := HocapG {
+  hocap_stateG :> inG Σ (authR (optionUR $ exclR (listO valO)));
+}.
+Definition hocapΣ : gFunctors :=
+  #[GFunctor (exclR unitO); GFunctor (authR (optionUR $ exclR (listO valO)))].
+
+Instance subG_hocapΣ {Σ} : subG hocapΣ Σ → hocapG Σ.
+Proof. solve_inG. Qed.
+
+Section hocap_pred_auth.
+  Context `{!heapG Σ} `{!hocapG Σ} (stack: hocap_pred.stack Σ).
+
+  Definition hocap_name : Type := gname.
+  Implicit Types γs : hocap_name.
+
+  Definition hocap_auth_stack_content_auth γs l : iProp Σ := own γs (● Excl' l).
+  Definition hocap_auth_stack_content_frag γs l : iProp Σ := own γs (◯ Excl' l).
+
+  Definition hocap_auth_is_stack N γs v : iProp Σ :=
+    stack.(hocap_pred.is_stack) N v (hocap_auth_stack_content_auth γs).
+
+  Lemma hocap_auth_new_stack N :
+    {{{ True }}}
+      stack.(hocap_pred.new_stack) #()
+    {{{ γs s, RET s; hocap_auth_is_stack N γs s ∗ hocap_auth_stack_content_frag γs [] }}}.
+  Proof.
+    iIntros (Φ) "_ HΦ". iApply wp_fupd.
+    iMod (own_alloc (● Excl' [] ⋅ ◯ Excl' [])) as (γs) "[Hs● Hs◯]".
+    { apply auth_both_valid. split; done. }
+    iApply (hocap_pred.new_stack_spec _ _ (hocap_auth_stack_content_auth γs) with "[Hs● //]").
+    iIntros "!>" (s) "#Hstack". iApply "HΦ".
+    rewrite /hocap_auth_is_stack. by iFrame.
+  Qed.
+
+  Lemma hocap_auth_push N γs s (v : val) (Φ : val → iProp Σ) :
+    hocap_auth_is_stack N γs s -∗
+    make_laterable (∀ l, hocap_auth_stack_content_auth γs l ={⊤∖↑N}=∗
+      hocap_auth_stack_content_auth γs (v::l) ∗ Φ #()) -∗
+    WP stack.(hocap_pred.push) s v {{ Φ }}.
+  Proof.
+    iIntros "#Hstack Hupd". iApply (hocap_pred.push_spec with "Hstack").
+    (* FIXME can we have proof mode support for make_laterable_intro? *)
+    iApply (laterable.make_laterable_intro with "[] Hupd"); iIntros "!# Hupd".
+    iIntros (l) ">Hs".
+    (* FIXME can we have proof mode support for make_laterable_elim? *)
+    iDestruct "Hupd" as ">Hupd". iDestruct (make_laterable_elim with "Hupd") as "Hupd".
+    iMod ("Hupd" with "Hs") as "[Hs $]". done.
+  Qed.
+
+  Lemma hocap_auth_pop N γs s (Φ : val → iProp Σ) :
+    hocap_auth_is_stack N γs s -∗
+    make_laterable (∀ l, hocap_auth_stack_content_auth γs l ={⊤∖↑N}=∗
+          match l with [] => hocap_auth_stack_content_auth γs [] ∗ Φ NONEV
+                | v :: l' => hocap_auth_stack_content_auth γs l' ∗ Φ (SOMEV v) end) -∗
+    WP stack.(hocap_pred.pop) s {{ Φ }}.
+  Proof.
+    iIntros "#Hstack Hupd". iApply (hocap_pred.pop_spec with "Hstack").
+    iApply (laterable.make_laterable_intro with "[] Hupd"); iIntros "!# Hupd".
+    iIntros (l) ">Hs".
+    iDestruct "Hupd" as ">Hupd". iDestruct (make_laterable_elim with "Hupd") as "Hupd".
+    iMod ("Hupd" with "Hs") as "HsΦ".
+    iModIntro. destruct l; iDestruct "HsΦ" as "[Hs HΦ]"; eauto with iFrame.
+  Qed.
+
+  Program Definition hocap_pred_auth : hocap_auth.stack Σ :=
+    {| hocap_auth.new_stack_spec := hocap_auth_new_stack;
+       hocap_auth.push_spec := hocap_auth_push;
+       hocap_auth.pop_spec := hocap_auth_pop |}.
+  Next Obligation.
+    iIntros (???) "Hf1 Hf2". iDestruct (own_valid_2 with "Hf1 Hf2") as %[].
+  Qed.
+  Next Obligation.
+    iIntros (???) "Ha1 Ha2". by iDestruct (own_valid_2 with "Ha1 Ha2") as %[].
+  Qed.
+  Next Obligation.
+    iIntros (???) "Hf Ha". iDestruct (own_valid_2 with "Ha Hf") as
+      %[->%Excl_included%leibniz_equiv _]%auth_both_valid. done.
+  Qed.
+  Next Obligation.
+    iIntros (???) "Hf Ha". iMod (own_update_2 with "Ha Hf") as "[? ?]".
+    { eapply auth_update, option_local_update, (exclusive_local_update _ (Excl _)). done. }
+    by iFrame.
+  Qed.
+
+End hocap_pred_auth.
+
+
 (** Show that our way of writing the [pop_spec] is equivalent to what is done in
-[concurrent_stack.spec].  IOW, the conjunction-vs-match doesn't matter.  Fixing
-the postcondition (the [Q] in [concurrent_stack.spec]) still matters. *)
+[concurrent_stack.spec].  IOW, the conjunction-vs-match doesn't matter. *)
 Section pop_equiv.
   Context `{invG Σ} (T : Type).
 
@@ -86,143 +380,3 @@ Section pop_equiv.
     - iIntros "HΦ" (l) "HI". destruct l; rewrite [(I _ ∗ _)%I]bi.sep_comm; by iApply "HΦ".
   Qed.
 End pop_equiv.
-
-(** From a HoCAP stack we can directly implement the logically atomic
-interface. *)
-Section hocap_logatom.
-  Context `{!heapG Σ} (stack: hocap_stack Σ).
-
-  Lemma logatom_push N γs s (v : val) :
-    stack.(is_stack) N γs s -∗
-    <<< ∀ l : list val, stack.(stack_content_frag) γs l >>>
-      stack.(push) s v @ ⊤∖↑N
-    <<< stack.(stack_content_frag) γs (v::l), RET #() >>>.
-  Proof.
-    iIntros "Hstack". iIntros (Φ) "HΦ".
-    iApply (push_spec with "Hstack").
-    iApply (make_laterable_intro with "[] HΦ"). iIntros "!# >HΦ" (l) "Hauth".
-    iMod "HΦ" as (l') "[Hfrag [_ Hclose]]".
-    iDestruct (stack_content_agree with "Hfrag Hauth") as %->.
-    iMod (stack_content_update with "Hfrag Hauth") as "[Hfrag $]".
-    iMod ("Hclose" with "Hfrag") as "HΦ". done.
-  Qed.
-
-  Lemma logatom_pop N γs (s : val) :
-    stack.(is_stack) N γs s -∗
-    <<< ∀ l : list val, stack.(stack_content_frag) γs l >>>
-      stack.(pop) s @ ⊤∖↑N
-    <<< stack.(stack_content_frag) γs (tail l),
-        RET match l with [] => NONEV | v :: _ => SOMEV v end >>>.
-  Proof.
-    iIntros "Hstack". iIntros (Φ) "HΦ".
-    iApply (pop_spec with "Hstack").
-    iApply (make_laterable_intro with "[] HΦ"). iIntros "!# >HΦ" (l) "Hauth".
-    iMod "HΦ" as (l') "[Hfrag [_ Hclose]]".
-    iDestruct (stack_content_agree with "Hfrag Hauth") as %->.
-    destruct l;
-    iMod (stack_content_update with "Hfrag Hauth") as "[Hfrag $]";
-    iMod ("Hclose" with "Hfrag") as "HΦ"; done.
-  Qed.
-
-  Definition hocap_logatom : logatom.atomic_stack Σ :=
-    {| logatom.new_stack_spec := stack.(new_stack_spec);
-       logatom.push_spec := logatom_push;
-       logatom.pop_spec := logatom_pop;
-       logatom.stack_content_exclusive := stack.(stack_content_frag_exclusive) |}.
-
-End hocap_logatom.
-
-(** From a logically atomic stack, we can implement a HoCAP stack by adding an
-auth invariant. *)
-
-(** The CMRA & functor we need. *)
-Class hocapG Σ := HocapG {
-  hocap_stateG :> inG Σ (authR (optionUR $ exclR (listO valO)));
-}.
-Definition hocapΣ : gFunctors :=
-  #[GFunctor (exclR unitO); GFunctor (authR (optionUR $ exclR (listO valO)))].
-
-Instance subG_hocapΣ {Σ} : subG hocapΣ Σ → hocapG Σ.
-Proof. solve_inG. Qed.
-
-Section logatom_hocap.
-  Context `{!heapG Σ} `{!hocapG Σ} (stack: logatom.atomic_stack Σ).
-
-  Definition hocap_name : Type := stack.(logatom.name) * gname.
-  Implicit Types γs : hocap_name.
-
-  Definition hocap_stack_content_auth γs l : iProp Σ := own γs.2 (● Excl' l).
-  Definition hocap_stack_content_frag γs l : iProp Σ := own γs.2 (◯ Excl' l).
-
-  Definition hocap_is_stack N γs v : iProp Σ :=
-    (stack.(logatom.is_stack) (N .@ "stack") γs.1 v ∗
-     inv (N .@ "wrapper") (∃ l, stack.(logatom.stack_content) γs.1 l ∗ hocap_stack_content_auth γs l))%I.
-
-  Lemma hocap_new_stack N :
-    {{{ True }}}
-      stack.(logatom.new_stack) #()
-    {{{ γs s, RET s; hocap_is_stack N γs s ∗ hocap_stack_content_frag γs [] }}}.
-  Proof.
-    iIntros (Φ) "_ HΦ". iApply wp_fupd. iApply logatom.new_stack_spec; first done.
-    iIntros "!>" (γs s) "[Hstack Hcont]".
-    iMod (own_alloc (● Excl' [] ⋅ ◯ Excl' [])) as (γw) "[Hs● Hs◯]".
-    { apply auth_both_valid. split; done. }
-    iApply ("HΦ" $! (γs, γw)). rewrite /hocap_is_stack. iFrame.
-    iApply inv_alloc. eauto with iFrame.
-  Qed.
-
-  Lemma hocap_push N γs s (v : val) (Φ : val → iProp Σ) :
-    hocap_is_stack N γs s -∗
-    make_laterable (∀ l, hocap_stack_content_auth γs l ={⊤∖↑N}=∗ hocap_stack_content_auth γs (v::l) ∗ Φ #()) -∗
-    WP stack.(logatom.push) s v {{ Φ }}.
-  Proof using Type*.
-    iIntros "#[Hstack Hwrap] Hupd". awp_apply (logatom.push_spec with "Hstack").
-    iInv "Hwrap" as (l) "[>Hcont >H●]".
-    iAaccIntro with "Hcont"; first by eauto 10 with iFrame.
-    iIntros "Hcont".
-    iMod fupd_intro_mask' as "Hclose";
-      last iMod (make_laterable_elim with "Hupd H●") as "[H● HΦ]"; first solve_ndisj.
-    iMod "Hclose" as "_". iIntros "!>".
-    eauto with iFrame.
-  Qed.
-
-  Lemma hocap_pop N γs s (Φ : val → iProp Σ) :
-    hocap_is_stack N γs s -∗
-    make_laterable (∀ l, hocap_stack_content_auth γs l ={⊤∖↑N}=∗
-          match l with [] => hocap_stack_content_auth γs [] ∗ Φ NONEV
-                | v :: l' => hocap_stack_content_auth γs l' ∗ Φ (SOMEV v) end) -∗
-    WP stack.(logatom.pop) s {{ Φ }}.
-  Proof using Type*.
-    iIntros "#[Hstack Hwrap] Hupd". awp_apply (logatom.pop_spec with "Hstack").
-    iInv "Hwrap" as (l) "[>Hcont >H●]".
-    iAaccIntro with "Hcont"; first by eauto 10 with iFrame.
-    iIntros "Hcont". destruct l.
-    - iMod fupd_intro_mask' as "Hclose";
-        last iMod (make_laterable_elim with "Hupd H●") as "[H● HΦ]"; first solve_ndisj.
-       iMod "Hclose" as "_". iIntros "!>"; eauto with iFrame.
-    - iMod fupd_intro_mask' as "Hclose";
-        last iMod (make_laterable_elim with "Hupd H●") as "[H● HΦ]"; first solve_ndisj.
-       iMod "Hclose" as "_". iIntros "!>"; eauto with iFrame.
-  Qed.
-
-  Program Definition logatom_hocap : hocap_stack Σ :=
-    {| new_stack_spec := hocap_new_stack;
-       push_spec := hocap_push;
-       pop_spec := hocap_pop |}.
-  Next Obligation.
-    iIntros (???) "Hf1 Hf2". iDestruct (own_valid_2 with "Hf1 Hf2") as %[].
-  Qed.
-  Next Obligation.
-    iIntros (???) "Ha1 Ha2". by iDestruct (own_valid_2 with "Ha1 Ha2") as %[].
-  Qed.
-  Next Obligation.
-    iIntros (???) "Hf Ha". iDestruct (own_valid_2 with "Ha Hf") as
-      %[->%Excl_included%leibniz_equiv _]%auth_both_valid. done.
-  Qed.
-  Next Obligation.
-    iIntros (???) "Hf Ha". iMod (own_update_2 with "Ha Hf") as "[? ?]".
-    { eapply auth_update, option_local_update, (exclusive_local_update _ (Excl _)). done. }
-    by iFrame.
-  Qed.
-
-End logatom_hocap.
